added further experiments to size of ATCs

ATC.thy
@@ -13,6 +13,121 @@ fun is_atc_reaction :: "('in, 'out, 'state) FSM \<Rightarrow> 'state \<Rightarro
   Some t \<Rightarrow> (x = xi \<and> (\<exists> s2 . (s1,xi,yi,s2) \<in> transitions M \<and> is_atc_reaction M s2 t io)) |
   None \<Rightarrow> (io = [] \<and> x = xi \<and> (\<exists> s2 . (s1,xi,yi,s2) \<in> transitions M)))"
 
+fun has_height_gte :: "('in, 'out) ATC \<Rightarrow> nat \<Rightarrow> bool" where
+"has_height_gte Leaf n = True" |
+"has_height_gte (Node x f) 0 = False" |
+"has_height_gte (Node x f) (Suc n) = (\<forall> t \<in> ran f .  has_height_gte t n)"
+(*"has_height_gte (Node x f) (Suc n) = Ball (ran f) (\<lambda> t . has_height_gte t n)"*)
+
+
+
+
+definition has_height :: "('in, 'out) ATC \<Rightarrow> nat \<Rightarrow> bool" where
+"has_height T n \<equiv> has_height_gte T n \<and> (\<forall> i < n . \<not> has_height_gte T i)"
+
+definition height :: "('in, 'out) ATC \<Rightarrow> nat" where
+"height T = (THE n . has_height T n)"
+
+fun atc_height :: "('in, 'out) ATC \<Rightarrow> nat" where
+"atc_height T = (LEAST n . has_height_gte T n)"
+
+lemma height_inc : "has_height_gte t n1 \<Longrightarrow> n2 > n1 \<Longrightarrow> has_height_gte t n2"
+proof (induction t  arbitrary: n1 n2)
+  case Leaf
+  then show ?case by simp
+next
+  case (Node x f)
+  have gtz : "n1 > 0"
+  proof (rule ccontr)
+    assume "\<not> (n1 > 0)"
+    then have "t = Leaf" using has_height_gte.elims(2) using Node.prems by blast
+    then show "False" using Node \<open>\<not> 0 < n1\<close> by auto
+  qed
+  have "\<forall> t1 \<in> ran f . has_height_gte t1 (n2-1)"
+  proof 
+    fix t1 
+    show "t1 \<in> ran f \<Longrightarrow> has_height_gte t1 (n2-1)"
+    proof (rule Node.IH [of "Some t1" "t1" "n1-1" "n2-1"])
+      assume el: "t1 \<in> ran f"
+      show "Some t1 \<in> range f" using el by (smt mem_Collect_eq ran_def rangeI)
+      show "t1 \<in> set_option (Some t1)" by auto
+      show "has_height_gte t1 (n1-1)" using Node.prems(1) gtz el gr0_conv_Suc by auto
+      show "(n2-1) > (n1-1)" using Node.prems(2) gtz by linarith
+    qed
+  qed
+  then show "has_height_gte (Node x f) n2" using Node.prems(2) diff_Suc_1 has_height_gte.elims(3) less_numeral_extra(3) by fastforce
+qed
+
+
+
+
+lemma height_ex : "\<exists> n . has_height_gte t n"
+proof (induction t)
+  case Leaf
+  then show ?case by auto
+next
+  case (Node x f)
+  have "\<forall> t1 \<in> ran f . \<exists> n1 . has_height_gte t1 n1" 
+    by (smt Node.IH UNIV_I image_eqI mem_Collect_eq option.set_intros ran_def)
+  then obtain hc where hc_def : "\<forall> t1 \<in> ran f . \<exists> n1 . has_height_gte t1 n1 \<and> n1 < hc" by sledgehamme
+  then obtain hs where hs_def : "\<forall> t1 \<in> ran f . has_height_gte t1 (hs t1)" by sledgehamme
+  then have "\<exists> n1 . \<forall> t1 \<in> ran f . has_height_gte t1 n1" using height_inc by sledgehamm
+  then show ?case by sledgehamme
+qed
+
+lemma test :
+  assumes a : "h1 = atc_height T"
+  shows "\<forall> i < h1 . \<not> has_height_gte T i"
+  using assms by sledgehamme
+
+lemma has_height_subtest :
+  assumes st: "t \<in> ran f"
+  assumes h1: "has_height t h1" 
+  assumes h2: "has_height (Node x f) t2"
+  shows "h2 > h1"
+  using assms by sledgehamme
+
+lemma has_height_subtest :
+  assumes st: "t \<in> ran f"
+  assumes h1: "h1 = atc_height t" 
+  assumes h2: "h2 = atc_height (Node x f)"
+  shows "h2 > h1"
+proof (rule ccontr)
+  assume "h2 \<le> h1"
+  then have "\<forall> i < h1 . \<not>(has_height_gte t i)" using assms by sledgehamme
+
+  then have "\<exists> t2 \<in> ran f . has_height_gte t2 n1" using assms by blast
+  then have "n2 > n1" using assms by sledgehamme
+  
+
+lemma subtest_height :
+  assumes st: "t \<in> ran f"
+  shows "atc_height t < atc_height (Node x f)"
+proof (rule ccontr)
+  assume "atc_height t \<ge> atc_height (Node x f)"
+  then obtain n where n_def : "n = atc_height (Node x f)" by auto
+  
+
+inductive subtest :: "('in, 'out) ATC \<Rightarrow> ('in, 'out) ATC \<Rightarrow> bool" where
+"t \<in> ran f \<Longrightarrow> subtest t (Node x f)"
+
+lemma accp_subtest : "Wellfounded.accp subtest t"
+proof (induction t)
+  case Leaf
+  then show ?case by (metis ATC.distinct(2) not_accp_down subtest.cases)
+next
+  case (Node x1 x2)
+  then show ?case by sledgehamme
+qed
+
+function size :: "('in, 'out) ATC \<Rightarrow> nat" where
+"size Leaf = 0" |
+"size (Node x f) = Max ( image size (ran f) )"
+  by pat_completeness auto
+termination 
+  apply (relation "measure atc_height")
+   apply auto[]
+  apply sledgehamme
 (*
 datatype ('in, 'out) ATC = Leaf | Node 'in "'out \<Rightarrow> nat" "('in, 'out) ATC list"
 
